dimsum_examples/r2a_bij_vertical2.v
@@ -1,0 +1,864 @@
+From dimsum.examples Require Import rec_to_asm2 rec_heap_inj.
+From dimsum.core.iris Require Import weak_embed sat.
+
+Set Default Proof Using "Type".
+Open Scope Z_scope.
+
+(** ** Definitions for combining and splitting injections *)
+(** abbreviation: r2av: rec_to_asm_vertical *)
+(** inj: source (rec) -> impl (asm), injb: source (rec) -> middle (rec), inja: middle (rec) -> impl (asm) *)
+
+(** [r2av_combine inja injb] combines the small injections [inja] and
+[injb] into a large injection *)
+Definition r2av_combine (inja : gmap prov Z) (injb : gmap prov loc) : gmap prov Z :=
+  omap (λ l, (λ ai, ai + l.2) <$> inja !! l.1) injb.
+
+(** [r2av_core_b inja injb] computes the part of [injb] that is also
+used by the large injection *)
+Definition r2av_core_b (inja : gmap prov Z) (injb : gmap prov loc) : gmap prov loc :=
+  filter (λ x, is_Some (inja !! x.2.1)) injb.
+
+(** [r2av_core_b inja injb] computes the part of [inja] that is also
+used by the large injection *)
+Definition r2av_core_a (inja : gmap prov Z) (injb : gmap prov loc) : gmap prov Z :=
+  filter (λ x, x.1 ∈ set_map (D:=gset _) fst (map_img (SA:=gset loc) injb)) inja.
+
+(** [r2av_proj_b inj inja injb X] projects a new b injection [injb'] injection
+from the large injection [inj]. It preserves the previous [injb] and
+allocates new provenances in the middle from outside [X]. *)
+Definition r2av_proj_b (inj inja : gmap prov Z) (injb : gmap prov loc) (X : gset prov) : gmap prov loc :=
+  injb ∪ ((λ p, (p, 0%Z)) <$> fresh_map (dom inj) X).
+
+(** [r2av_proj_a inj inja injb X] projects a new a injection [inja'] injection
+from the large injection [inj]. It preserves the previous [inja] and
+allocates new provenances in the middle from outside [X]. *)
+Definition r2av_proj_a (inj inja : gmap prov Z) (injb : gmap prov loc) (X : gset prov) : gmap prov Z :=
+  inja ∪ kmap (λ p, fresh_map (dom inj) X !!! p) (inj ∖ gset_to_gmap 0 (dom injb)).
+
+(** [r2av_residual] is what is left in the middle heap after the
+small injections are converted to large injection. *)
+Definition r2av_residual {Σ} `{!satG Σ heap_injUR} `{!satG Σ rec_to_asmUR} (γa γb : sat_name _) (l : loc) : iProp Σ :=
+  ∃ b, ⌜l.2 = 0⌝ ∗ ⌈l.1 ↦∗hi b @ sat γb⌉ ∗ ⌈l.1 ↦∗h b @ sat γa⌉.
+
+(** *** Lookup lemmas *)
+Lemma r2av_combine_lookup_Some inja injb ps ai0:
+  r2av_combine inja injb !! ps = Some ai0 ↔
+   ∃ l ai', injb !! ps = Some l ∧ inja !! l.1 = Some ai' ∧ ai0 = ai' + l.2.
+Proof.
+  rewrite /r2av_combine lookup_omap_Some. f_equiv => ? /=.
+  rewrite fmap_Some. naive_solver.
+Qed.
+
+Lemma r2av_core_b_lookup_Some inja injb p l :
+  r2av_core_b inja injb !! p = Some l ↔
+   injb !! p = Some l ∧ is_Some (inja !! l.1).
+Proof. by rewrite /r2av_core_b map_lookup_filter_Some. Qed.
+
+Lemma r2av_core_b_lookup_None inja injb p :
+  r2av_core_b inja injb !! p = None ↔
+   (∀ l, injb !! p = Some l → inja !! l.1 = None).
+Proof.
+  rewrite eq_None_not_Some /is_Some.
+  setoid_rewrite r2av_core_b_lookup_Some. split.
+  2: rewrite /is_Some; naive_solver.
+  move => Hl l ?. apply eq_None_not_Some. naive_solver.
+Qed.
+
+Lemma r2av_core_a_lookup_Some inja injb p a :
+  r2av_core_a inja injb !! p = Some a ↔
+   inja !! p = Some a ∧ ∃ ps lm, injb !! ps = Some lm ∧ lm.1 = p.
+Proof.
+  rewrite /r2av_core_a map_lookup_filter_Some /=.
+  rewrite elem_of_map. setoid_rewrite elem_of_map_img.
+  naive_solver.
+Qed.
+
+Lemma r2av_proj_b_lookup_Some inj inja injb X p (l : loc) :
+  r2av_proj_b inj inja injb X !! p = Some l ↔
+   injb !! p = Some l ∨ injb !! p = None ∧
+     fresh_map (dom inj) X !! p = Some l.1 ∧ l.2 = 0.
+Proof.
+  rewrite /r2av_proj_b lookup_union_Some_raw. do 2 f_equiv.
+  rewrite lookup_fmap_Some. destruct l; naive_solver.
+Qed.
+
+Lemma r2av_proj_a_lookup_Some inj inja injb X p a :
+  r2av_proj_a inj inja injb X !! p = Some a ↔
+   inja !! p = Some a ∨ inja !! p = None ∧
+     ∃ ps, inj !! ps = Some a ∧ injb !! ps = None ∧ fresh_map (dom inj) X !! ps = Some p.
+Proof.
+  rewrite /r2av_proj_a lookup_union_Some_raw. do 2 f_equiv.
+  rewrite lookup_kmap_Some_strong. 2: {
+    move => i j [?/lookup_difference_Some[??]] [?/lookup_difference_Some[??]].
+    rewrite !lookup_total_alt.
+    destruct (fresh_map (dom inj) X !! i) eqn:Heq. 2: {
+      move: Heq => /fresh_map_lookup_None/not_elem_of_dom. naive_solver. }
+    destruct (fresh_map (dom inj) X !! j) eqn:Heq2. 2: {
+      move: Heq2 => /fresh_map_lookup_None/not_elem_of_dom. naive_solver. }
+    move => ?. simplify_eq/=. apply (fresh_map_bij _ _ _ _ _ Heq Heq2).
+  }
+  f_equiv => ?. rewrite lookup_difference_Some lookup_gset_to_gmap_None not_elem_of_dom.
+  split => -[??]; destruct!; split!; subst.
+  - apply lookup_lookup_total. by apply fresh_map_lookup_is_Some, elem_of_dom.
+  - by erewrite lookup_total_correct.
+Qed.
+
+
+(** *** Lemmas about the definitions  *)
+(** [r2av_combine] is monotonic. *)
+Lemma r2av_combine_subseteq inja injb inja' injb':
+  inja ⊆ inja' →
+  injb ⊆ injb' →
+  r2av_combine inja injb ⊆ r2av_combine inja' injb'.
+Proof.
+  move => Hsuba Hsubb. apply map_subseteq_spec => ??.
+  rewrite !r2av_combine_lookup_Some.
+  move => [? [? [/(lookup_weaken _ _ _ _)/(_ Hsubb)? [/(lookup_weaken _ _ _ _)/(_ Hsuba) ??]]]].
+  naive_solver.
+Qed.
+
+(** [r2av_core_a] is smaller than [inja] *)
+Lemma r2av_core_a_subseteq inja injb :
+  r2av_core_a inja injb ⊆ inja.
+Proof. apply map_subseteq_spec => ?? /r2av_core_a_lookup_Some. naive_solver. Qed.
+
+(** [r2av_core_b] is smaller than [inja] *)
+Lemma r2av_core_b_subseteq inja injb :
+  r2av_core_b inja injb ⊆ injb.
+Proof. apply map_subseteq_spec => ?? /r2av_core_b_lookup_Some. naive_solver. Qed.
+
+(** [r2av_proj_a] is bigger than [inja] *)
+Lemma r2av_proj_a_subseteq inj inja injb X :
+  inja ⊆ r2av_proj_a inj inja injb X.
+Proof. apply map_union_subseteq_l. Qed.
+
+(** [r2av_proj_b] is bigger than [injb] *)
+Lemma r2av_proj_b_subseteq inj inja injb X :
+  injb ⊆ r2av_proj_b inj inja injb X.
+Proof. apply map_union_subseteq_l. Qed.
+
+(** We can convert the new large injection [inj] as a combination of
+the projections. *)
+Lemma r2av_combine_proj inj inja injb X :
+  (** inj only grew *)
+  r2av_combine inja injb ⊆ inj →
+  (** inj does have provs that are already in injb (except for those in the core) *)
+  (** We do not need a similar assumption for inja since it is fine to map multiple
+    source provs to the same target *)
+  dom inj ## dom (injb ∖ r2av_core_b inja injb) →
+  (** newly allocated provs must be disjoint from the existing ones in inja and injb *)
+  dom inja ⊆ X →
+  map_img (fst <$> injb) ⊆ X →
+  inj = r2av_combine (r2av_proj_a inj inja injb X) (r2av_proj_b inj inja injb X).
+Proof.
+  move => Hsub Hdisj HXa HXb.
+  apply map_eq => p. apply option_eq => li.
+  rewrite r2av_combine_lookup_Some.
+  setoid_rewrite r2av_proj_a_lookup_Some.
+  setoid_rewrite r2av_proj_b_lookup_Some.
+  split => Hp.
+  - have : (injb ∖ r2av_core_b inja injb) !! p = None.
+    { apply not_elem_of_dom. apply: Hdisj. by apply elem_of_dom. }
+    move => /lookup_difference_None[?|[?/r2av_core_b_lookup_Some[?[??]]]].
+    + have [??]: is_Some (fresh_map (dom inj) X !! p) by apply fresh_map_lookup_is_Some, elem_of_dom.
+      eexists (_, _), _. split!. 2: by rewrite Z.add_0_r. right.
+      split! => //. exploit @fresh_map_lookup_Some; [done|]. move => [_ Hnotin].
+      apply eq_None_not_Some => -[?]. contradict Hnotin. apply HXa.
+      by apply elem_of_dom.
+    + move: Hsub =>/map_subseteq_spec Hsub.
+      exploit Hsub. { apply r2av_combine_lookup_Some. naive_solver. }
+      naive_solver.
+  - destruct!.
+    + move: Hsub =>/map_subseteq_spec Hsub. apply Hsub.
+      apply r2av_combine_lookup_Some. naive_solver.
+    + exploit @fresh_map_lookup_Some; [done|]. move => [_ Hnotin].
+      contradict Hnotin. apply HXa. by apply elem_of_dom.
+    + exploit @fresh_map_lookup_Some; [done|]. move => [_ Hnotin].
+      contradict Hnotin. apply HXb, elem_of_map_img. eexists _.
+      apply lookup_fmap_Some. naive_solver.
+    + have ? : p = ps by apply: fresh_map_bij. rewrite H5 Z.add_0_r. naive_solver.
+Qed.
+
+(** The core of a only grows. *)
+Lemma r2av_core_a_proj_subseteq inja injb inj X :
+  r2av_core_a inja injb ⊆ r2av_core_a (r2av_proj_a inj inja injb X) (r2av_proj_b inj inja injb X).
+Proof.
+  apply map_subseteq_spec => ?? /r2av_core_a_lookup_Some [? [? [? [??]]]].
+  apply r2av_core_a_lookup_Some. split.
+  - apply r2av_proj_a_lookup_Some. naive_solver.
+  - eexists _, _. split; [|done]. apply r2av_proj_b_lookup_Some. naive_solver.
+Qed.
+
+
+(** The core of b only grows. *)
+Lemma r2av_core_b_proj_subseteq inja injb inj X :
+  r2av_core_b inja injb ⊆ r2av_core_b (r2av_proj_a inj inja injb X) (r2av_proj_b inj inja injb X).
+Proof.
+  apply map_subseteq_spec => ?? /r2av_core_b_lookup_Some [? [??]].
+  apply r2av_core_b_lookup_Some. split.
+  - apply r2av_proj_b_lookup_Some. naive_solver.
+  - eexists _. apply r2av_proj_a_lookup_Some. naive_solver.
+Qed.
+
+
+(** This lemma allows us to build the new a injection [inja'] by
+replacing the core of [inja]. (Technically, we only need the right to
+left inclusion.) *)
+Lemma r2av_recombine_a inja injb inja' injb' inj' X :
+  inja' = r2av_proj_a inj' inja injb X →
+  injb' = r2av_proj_b inj' inja injb X →
+  (inja ∖ r2av_core_a inja injb ∪ r2av_core_a inja' injb') = inja'.
+Proof.
+  move => -> ->.
+  apply map_eq => pm. apply option_eq => li.
+  rewrite lookup_union_Some_raw lookup_difference_Some lookup_difference_None.
+  split.
+  - move => [[??]| [? /r2av_core_a_lookup_Some [??]]] //.
+    apply: lookup_weaken; [done|]. apply r2av_proj_a_subseteq.
+  - move => /r2av_proj_a_lookup_Some[?|[?[?[?[??]]]]].
+    + destruct (r2av_core_a inja injb !! pm) eqn:Heq; [|naive_solver]. split!.
+      apply: lookup_weaken. 2: apply r2av_core_a_proj_subseteq.
+      move: (Heq) => /r2av_core_a_lookup_Some. naive_solver.
+    + split!. by left. apply r2av_core_a_lookup_Some. split.
+      * apply r2av_proj_a_lookup_Some. naive_solver.
+      * eexists _, (_, _). split!. apply r2av_proj_b_lookup_Some. by right.
+Qed.
+
+(** This lemma allows us to build the new a injection [injb'] by
+replacing the core of [injb]. (Technically, we only need the right to
+left inclusion.) *)
+Lemma r2av_recombine_b inja injb inja' injb' inj' X :
+  inja' = r2av_proj_a inj' inja injb X →
+  injb' = r2av_proj_b inj' inja injb X →
+  dom inja ⊆ X →
+  (injb ∖ r2av_core_b inja injb ∪ r2av_core_b inja' injb') = injb'.
+Proof.
+  move => -> -> HXa.
+  apply map_eq => ps. apply option_eq => lm.
+  rewrite lookup_union_Some_raw lookup_difference_Some lookup_difference_None.
+  rewrite r2av_core_b_lookup_None r2av_core_b_lookup_Some.
+  split.
+  - move => [[??]|[?[??]]] //. apply: lookup_weaken; [done|].
+    apply r2av_proj_b_subseteq.
+  - move => /r2av_proj_b_lookup_Some[?|[?[??]]].
+    + destruct (inja !! lm.1) eqn:?.
+      * right. split!. { eexists _. apply r2av_core_b_lookup_Some. naive_solver. }
+        { apply r2av_proj_b_lookup_Some. naive_solver. }
+        eexists _. apply r2av_proj_a_lookup_Some. by left.
+      * left. split!. move => ??. unfold loc in *. by simplify_eq.
+    + split!. by left.
+      * apply r2av_proj_b_lookup_Some. naive_solver.
+      * exploit @fresh_map_lookup_Some; [done|].
+        move => [/elem_of_dom[??] Hnotin]. eexists _.
+        apply r2av_proj_a_lookup_Some. right. split! => //.
+        apply eq_None_not_Some => -[?]. contradict Hnotin. apply HXa.
+        by apply elem_of_dom.
+Qed.
+
+(** [r2av_combine_to_b] allows us to express [r2av_combine] in terms of [r2av_core_b]. *)
+Lemma r2av_combine_to_b inja injb :
+  r2av_combine inja injb = (λ l, inja !!! l.1 + l.2) <$> r2av_core_b inja injb.
+Proof.
+  apply map_eq => ?. apply option_eq => ?. rewrite r2av_combine_lookup_Some.
+  rewrite lookup_fmap_Some. setoid_rewrite r2av_core_b_lookup_Some.
+  rewrite /is_Some. split => ?; destruct!/=; split!.
+  - by erewrite lookup_total_correct.
+  - by erewrite lookup_total_correct.
+Qed.
+
+(** provs in the new core that are not in the old core are fresh *)
+Lemma r2av_core_b_proj_fresh inj inja injb X p (l : loc):
+  map_img (fst <$> injb) ⊆ X →
+  (r2av_core_b (r2av_proj_a inj inja injb X) (r2av_proj_b inj inja injb X) ∖
+     r2av_core_b inja injb) !! p = Some l →
+  fresh_map (dom inj) X !! p = Some l.1 ∧ l.2 = 0.
+Proof.
+  move => HXb /lookup_difference_Some[/r2av_core_b_lookup_Some[/r2av_proj_b_lookup_Some Horb [? /r2av_proj_a_lookup_Some Hora]] /r2av_core_b_lookup_None?].
+  destruct Horb as [|[?[??]]]; [|done].
+  destruct Hora as [|[? [?[? [??]]]]]; [naive_solver|].
+  exploit @fresh_map_lookup_Some; [done|]. move => [? Hnotin]. contradict Hnotin. apply HXb. apply elem_of_map_img.
+  setoid_rewrite lookup_fmap_Some. naive_solver.
+Qed.
+
+Section vertical.
+Context {Σ} `{!satG Σ heap_injUR} `{!satG Σ rec_to_asmUR}.
+
+(** Combine the value relation. *)
+Lemma r2av_combine_val inja' injb' γa γb γ vi vm vs:
+  r2a_f2i_trader (sat γ) (sat γa) -∗
+  ⌈r2a_shared_auth inja' @ sat γa⌉ -∗
+  ⌈heap_inj_shared_auth injb' @ sat γb⌉ -∗
+  ⌈[∗ map] ps↦li0 ∈ r2av_combine inja' injb', r2a_shared ps li0 @ sat γ⌉ -∗
+  ⌈r2a_val_rel vm vi @ sat γa⌉ -∗
+  ⌈val_in_inj vm vs @ sat γb⌉ -∗
+  ⌈r2a_val_rel vs vi @ sat γ⌉.
+Proof.
+  iIntros "Ht Ha Hb H Hva Hvb".
+  iDestruct (r2a_f2i_trader_switch with "Ht") as "Ht".
+  destruct vm, vs => /=; rewrite ?weak_embed_pure //; iDestruct! => //.
+  - iApply (r2a_f2i_trade_incl with "[$] [$]").
+  - iDestruct "Hva" as (??) "Hla".
+    iDestruct "Hvb" as (??) "Hlb". subst => /=.
+    iDestruct (r2a_shared_lookup with "Ha [$]") as %?.
+    iDestruct (heap_inj_shared_lookup with "Hb [$]") as %?.
+    rewrite weak_embed_big_sepM.
+    iDestruct (big_sepM_lookup with "[$]") as "?".
+    { apply r2av_combine_lookup_Some. by split!. }
+    rewrite /loc_in_inj weak_embed_exist.
+    iExists _. iFrame. by rewrite Z.add_assoc.
+Qed.
+
+Lemma r2av_combine_val_list inja' injb' γa γb γ vi vm vs:
+  r2a_f2i_trader (sat γ) (sat γa) -∗
+  ⌈r2a_shared_auth inja' @ sat γa⌉ -∗
+  ⌈heap_inj_shared_auth injb' @ sat γb⌉ -∗
+  ⌈[∗ map] ps↦li0 ∈ r2av_combine inja' injb', r2a_shared ps li0 @ sat γ⌉ -∗
+  ⌈[∗ list] v1;v2∈vm;vi, r2a_val_rel v1 v2 @ sat γa⌉ -∗
+  ⌈[∗ list] v1;v2∈vm;vs, val_in_inj v1 v2 @ sat γb⌉ -∗
+  ⌈[∗ list] v1;v2∈vs;vi, r2a_val_rel v1 v2 @ sat γ⌉.
+Proof.
+  iIntros "#? Haa Hab ? Him Hms".
+  iInduction vm as [|] "IH" forall (vi vs). {
+    iDestruct (big_sepL2_nil_inv_l (PROP:=uPred rec_to_asmUR) with "Him") as %->.
+    iDestruct (big_sepL2_nil_inv_l (PROP:=uPred heap_injUR) with "Hms") as %->.
+    simpl. by iPureIntro.
+  }
+  iDestruct (big_sepL2_cons_inv_l (PROP:=uPred heap_injUR) with "Hms") as (?? ->) "[??]".
+  iDestruct (big_sepL2_cons_inv_l (PROP:=uPred rec_to_asmUR) with "Him") as (?? ->) "[??]".
+  simpl.
+  iDestruct (r2av_combine_val with "[$] Haa Hab [$] [$] [$]") as "#?".
+  iSplit; [done|]. iApply ("IH" with "[$] [$] [$] [$] [$]").
+Qed.
+
+Lemma r2av_combine_val_map `{Countable K} inja' injb' γa γb γ (vi vm vs : gmap K _):
+  r2a_f2i_trader (sat γ) (sat γa) -∗
+  ⌈r2a_shared_auth inja' @ sat γa⌉ -∗
+  ⌈heap_inj_shared_auth injb' @ sat γb⌉ -∗
+  ⌈[∗ map] ps↦li0 ∈ r2av_combine inja' injb', r2a_shared ps li0 @ sat γ⌉ -∗
+  ⌈[∗ map] v1;v2∈vi;vm, r2a_val_rel v2 v1 @ sat γa⌉ -∗
+  ⌈[∗ map] v1;v2∈vm;vs, val_in_inj v1 v2 @ sat γb⌉ -∗
+  ⌈[∗ map] v1;v2∈vi;vs, r2a_val_rel v2 v1 @ sat γ⌉.
+Proof.
+  iIntros "#? Haa Hab ? Him Hms".
+  iInduction vm as [|] "IH" using map_ind forall (vi vs). {
+    iDestruct (big_sepM2_empty_l (PROP:=uPred rec_to_asmUR) with "Him") as %->.
+    iDestruct (big_sepM2_empty_r (PROP:=uPred heap_injUR) with "Hms") as %->.
+    by rewrite big_sepM2_empty.
+  }
+  iDestruct (big_sepM2_delete_l (PROP:=uPred heap_injUR) with "Hms") as (??) "[??]".
+  { apply lookup_insert. }
+  iDestruct (big_sepM2_delete_r (PROP:=uPred rec_to_asmUR) with "Him") as (??) "[??]".
+  { apply lookup_insert. }
+  rewrite delete_insert //.
+  iDestruct (r2av_combine_val with "[$] Haa Hab [$] [$] [$]") as "#?".
+  erewrite <-(insert_delete vi) at 2; [|done].
+  erewrite <-(insert_delete vs) at 2; [|done].
+  rewrite big_sepM2_insert; simplify_map_eq => //.
+  iSplit; [done|]. iApply ("IH" with "[$] [$] [$] [$] [$]").
+Qed.
+
+(** Split the value relation. *)
+Lemma r2av_split_val inja' injb' γa γb γ vi vs:
+  r2a_f2i_trader (sat γ) (sat γa) -∗
+  ⌈[∗ map] ps↦li0 ∈ inja', r2a_shared ps li0 @ sat γa⌉ -∗
+  ⌈[∗ map] ps↦li0 ∈ injb', heap_inj_shared ps li0 @ sat γb⌉ -∗
+  ⌈r2a_shared_auth (r2av_combine inja' injb') @ sat γ⌉ -∗
+
+  ⌈r2a_val_rel vs vi @ sat γ⌉ -∗
+  ∃ vm, ⌈r2a_val_rel vm vi @ sat γa⌉ ∗ ⌈val_in_inj vm vs @ sat γb⌉.
+Proof.
+  iIntros "? Ha Hb H Hv".
+  destruct vs => /=; rewrite ?weak_embed_pure //; iDestruct!.
+  - iExists (ValNum _) => /=. by iPureIntro.
+  - iExists (ValBool _) => /=. by iPureIntro.
+  - iExists (ValFn _) => /=. iSplit; [|done]. iApply (r2a_f2i_trade_incl with "[$] [$]").
+  - iDestruct "Hv" as (li ?) "Hl".
+    iDestruct (r2a_shared_lookup with "H [$]") as %[lm[li'[?[??]]]]%r2av_combine_lookup_Some.
+    iDestruct (big_sepM_lookup (PROP:=uPred rec_to_asmUR) with "Ha") as "?"; [done|].
+    iDestruct (big_sepM_lookup (PROP:=uPred heap_injUR) with "Hb") as "?"; [done|].
+    subst. iExists (ValLoc (lm +ₗ l.2)) => /=. iFrame. iSplit; [|done].
+    unfold loc_in_inj. simpl. iFrame. by rewrite Z.add_assoc.
+Qed.
+
+Lemma r2av_split_val_list inja' injb' γa γb γ vis vss:
+  r2a_f2i_trader (sat γ) (sat γa) -∗
+  ⌈[∗ map] ps↦li0 ∈ inja', r2a_shared ps li0 @ sat γa⌉ -∗
+  ⌈[∗ map] ps↦li0 ∈ injb', heap_inj_shared ps li0 @ sat γb⌉ -∗
+  ⌈r2a_shared_auth (r2av_combine inja' injb') @ sat γ⌉ -∗
+
+  ⌈[∗ list] vi;vs∈vss;vis, r2a_val_rel vi vs @ sat γ⌉ -∗
+  ∃ vms, ⌈[∗ list] vi;vm∈vms;vis, r2a_val_rel vi vm @ sat γa⌉ ∗
+         ⌈[∗ list] vm;vs∈vms;vss, val_in_inj vm vs @ sat γb⌉.
+Proof.
+  iIntros "#? Ha Hb H Hv".
+  iInduction vis as [|] "IH" forall (vss). {
+    iDestruct (big_sepL2_nil_inv_r (PROP:=uPred rec_to_asmUR) with "Hv") as %->.
+    iExists []. by simpl.
+  }
+  iDestruct (big_sepL2_cons_inv_r (PROP:=uPred rec_to_asmUR) with "Hv") as (?? ->) "[??]".
+  iDestruct (r2av_split_val with "[$] Ha Hb [$] [$]") as (?) "#[??]".
+  iDestruct ("IH" with "Ha Hb [$] [$]") as (?) "#[??]".
+  iExists (_::_) => /=. by repeat iSplit.
+Qed.
+
+Lemma r2av_split_val_map {A} `{Countable A} inja' injb' γa γb γ (vis vss : gmap A _):
+  r2a_f2i_trader (sat γ) (sat γa) -∗
+  ⌈[∗ map] ps↦li0 ∈ inja', r2a_shared ps li0 @ sat γa⌉ -∗
+  ⌈[∗ map] ps↦li0 ∈ injb', heap_inj_shared ps li0 @ sat γb⌉ -∗
+  ⌈r2a_shared_auth (r2av_combine inja' injb') @ sat γ⌉ -∗
+
+  ⌈[∗ map] vi;vs∈vis;vss, r2a_val_rel vs vi @ sat γ⌉ -∗
+  ∃ vms, ⌈[∗ map] vi;vm∈vis;vms, r2a_val_rel vm vi @ sat γa⌉ ∗
+         ⌈[∗ map] vm;vs∈vms;vss, val_in_inj vm vs @ sat γb⌉.
+Proof.
+  iIntros "#? Ha Hb H Hv".
+  iInduction vis as [|] "IH" using map_ind forall (vss). {
+    iDestruct (big_sepM2_empty_r (PROP:=uPred rec_to_asmUR) with "Hv") as %->.
+    iExists ∅. by rewrite !big_sepM2_empty.
+  }
+  iDestruct (big_sepM2_delete_l (PROP:=uPred rec_to_asmUR) with "Hv") as (??) "[??]".
+  { apply lookup_insert. }
+  rewrite delete_insert //.
+  iDestruct (r2av_split_val with "[$] Ha Hb [$] [$]") as (?) "#[? ?]".
+  iEval (erewrite <-(insert_delete vss); [|done]).
+  iDestruct ("IH" with "[$] [$] [$] [$]") as (vms) "[??]".
+  iExists (<[_:=_]>vms). iSplit.
+  - by iApply (big_sepM2_insert_2 (PROP:=uPred rec_to_asmUR)); [done|].
+  - by iApply (big_sepM2_insert_2 (PROP:=uPred heap_injUR)); [done|].
+Qed.
+
+(** Allocate the residual for the new provs in the middle heap. *)
+Lemma r2av_alloc_residual (m : gmap prov loc) hm γa γb:
+  map_img (fst <$> m) ## h_provs hm →
+  (∀ i j k, (fst <$> m) !! i = Some k → (fst <$> m) !! j = Some k → i = j) →
+  (∀ i k, m !! i = Some k → k.2 = 0%Z) →
+  (filter is_ProvStatic (map_img (SA:=gset _) (fst <$> m)) = ∅) →
+  ⌈{sat γa}⌉ -∗ ⌈{sat (M:=heap_injUR) γb}⌉ -∗
+  ⌈r2a_heapUR_inv hm @ sat γa⌉ -∗
+  ⌈heap_inj_inv_i hm @ sat γb⌉ ==∗
+  ∃ hm', ([∗ map] li0 ∈ m, r2av_residual γa γb li0) ∗
+  ⌈{sat γa}⌉ ∗ ⌈{sat γb}⌉ ∗
+  ⌈r2a_heapUR_inv hm' @ sat γa⌉ ∗
+  ⌈heap_inj_inv_i hm' @ sat γb⌉ ∗
+  ⌜h_static_provs hm' = h_static_provs hm⌝.
+Proof.
+  iIntros (? Hinj Hm0 Hs) "?? Hinva Hinvb".
+
+  set bs : gmap prov (gmap Z val) := gset_to_gmap ∅ (map_img (fst <$> m)).
+  have ? : dom bs ## h_provs hm by rewrite dom_gset_to_gmap.
+
+  iApply (weak_embed_bupd_intro (sat γa) with "[$]").
+  iMod (heapUR_alloc_blocks r2a_heap bs with "Hinva") as "[? Ha]" => //.
+  iIntros "!> ?".
+  iApply (weak_embed_bupd_intro (sat γb) with "[$]").
+  iMod (heapUR_alloc_blocks own_heap_i bs with "Hinvb") as "[? Hb]" => //.
+  iIntros "!> ? !>". iFrame. iSplit. 2: {
+    iPureIntro. rewrite h_static_provs_heap_merge h_static_provs_heap_from_blocks.
+    rewrite dom_gset_to_gmap Hs. set_solver.
+  }
+  rewrite !big_sepM_gset_to_gmap !big_sepS_map_img_1 // !big_sepM_fmap.
+  rewrite !weak_embed_big_sepM.
+  iDestruct (big_sepM_sep_2 with "Ha Hb") as "?".
+  iApply (big_sepM_impl with "[$]"). iIntros "!>" (???) "[??]". iExists _. iFrame.
+  iPureIntro. by apply: Hm0.
+Qed.
+
+(** This lemma allows us to integrate the [big_sepM] over
+[r2av_core_a] into the [big_sepM] for [r2av_core_b]. This is useful
+since then we only need to do an induction over [r2av_core_b].
+However, this only holds if [r2av_core_b] is an injection, i.e. it
+maps different source provenances to different provenances in the
+middle heap. (Otherwise, we would need to reuse the same [Φa l.1 li]
+for multiple elements of [r2av_core_b]./) *)
+Lemma big_sepM_r2av_core_a_b_1 {PROP : bi} inja injb (Φa Φb : _ → _ → PROP) `{!BiAffine PROP} `{!BiPureForall PROP}:
+  (** Check that r2av_core_b is injective *)
+  (∀ p1 p2 l1 l2, ⌜l1.1 = l2.1⌝ -∗ Φb p1 l1 -∗ Φb p2 l2 -∗ False) -∗
+  ([∗ map] p↦l ∈ r2av_core_a inja injb, Φa p l) -∗
+  ([∗ map] p↦l ∈ r2av_core_b inja injb, Φb p l) -∗
+  ([∗ map] p↦l ∈ r2av_core_b inja injb,
+    Φb p l ∗ ∃ li, ⌜r2av_core_a inja injb !! l.1 = Some li⌝ ∗ Φa l.1 li).
+Proof.
+  iIntros "Hf ? Hb".
+  iAssert ⌜∀ p1 p2 l1 l2, l1.1 = l2.1 → r2av_core_b inja injb !! p1 = Some l1 → r2av_core_b inja injb !! p2 = Some l2 → p1 = p2⌝%I as %Himpl. {
+    iIntros (p1 p2 l1 l2 ? ??). destruct (decide (p1 = p2)) => //.
+    rewrite (big_sepM_delete _ (r2av_core_b _ _)); [|done]. iDestruct "Hb" as "[? Hb]".
+    iDestruct (big_sepM_lookup with "Hb") as "?". { apply lookup_delete_Some. naive_solver. }
+    iDestruct ("Hf" with "[//] [$] [$]") as %[].
+  }
+  iApply big_sepM_sep. iFrame.
+  iApply (big_sepM_impl_rel (λ pa la pb lb, pa = lb.1) with "[$]").
+  move => ?? /r2av_core_b_lookup_Some[?[??]].
+  split!.
+  - apply r2av_core_a_lookup_Some. naive_solver.
+  - iIntros "$". iPureIntro. apply r2av_core_a_lookup_Some. naive_solver.
+  - move => ????. apply: Himpl; [done| |done]. apply r2av_core_b_lookup_Some. naive_solver.
+Qed.
+
+Lemma big_sepM_r2av_core_a_b_2 {PROP : bi} inja injb (Φa Φb : _ → _ → PROP) `{!BiAffine PROP}:
+  ([∗ map] p↦l ∈ r2av_core_b inja injb,
+    Φb p l ∗ ∃ li, ⌜r2av_core_a inja injb !! l.1 = Some li⌝ ∗ Φa l.1 li) ⊢
+  ([∗ map] p↦l ∈ r2av_core_a inja injb, Φa p l) ∗
+  ([∗ map] p↦l ∈ r2av_core_b inja injb, Φb p l).
+Proof.
+  iIntros "Hb".
+  iDestruct (big_sepM_sep with "Hb") as "[$ ?]".
+  iApply (big_sepM_impl_rel (λ pb lb pa la, pa = lb.1) with "[$]").
+  move => ?? /r2av_core_a_lookup_Some[?[? [? [??]]]].
+  split!.
+  - done.
+  - apply r2av_core_b_lookup_Some. naive_solver.
+  - iIntros "(%& %Ha & ?)". move: Ha => /r2av_core_a_lookup_Some[?[?[?[??]]]]. by simplify_eq.
+  - naive_solver.
+Qed.
+
+Lemma big_sepM_r2av_core_a_b {PROP : bi} inja injb (Φa Φb : _ → _ → PROP) `{!BiAffine PROP} `{!BiPureForall PROP}:
+  (∀ p1 p2 l1 l2, l1.1 = l2.1 → Φb p1 l1 -∗ Φb p2 l2 -∗ False) →
+  ([∗ map] p↦l ∈ r2av_core_a inja injb, Φa p l) ∗
+  ([∗ map] p↦l ∈ r2av_core_b inja injb, Φb p l) ⊣⊢
+  ([∗ map] p↦l ∈ r2av_core_b inja injb,
+    Φb p l ∗ ∃ li, ⌜r2av_core_a inja injb !! l.1 = Some li⌝ ∗ Φa l.1 li).
+Proof.
+  move => Hf. iSplit.
+  - iIntros "[??]". iApply (big_sepM_r2av_core_a_b_1 with "[] [$] [$]"). iIntros. by iApply (Hf with "[$] [$]").
+  - iIntros "?". by iApply big_sepM_r2av_core_a_b_2.
+Qed.
+
+(** Create the large invariant and the residual from the two small invariants. *)
+Lemma r2av_shared_from_ab inja' injb' γa γb γ ha hb hm:
+  r2a_f2i_trader (sat γ) (sat γa) -∗
+  memUR_trader (sat γ) (sat γa) r2a_mem r2a_mem -∗
+  heapUR_trader (sat γ) (sat γb) r2a_heap own_heap_s -∗
+  ⌈r2a_memUR_inv ha @ sat γa⌉ -∗
+  ⌈r2a_heapUR_inv hm @ sat γa⌉ -∗
+  ⌈heap_inj_inv_i hm @ sat γb⌉ -∗
+  ⌈heap_inj_inv_s hb @ sat γb⌉ -∗
+  ⌈r2a_shared_auth inja' @ sat γa⌉ -∗
+  ⌈heap_inj_shared_auth injb' @ sat γb⌉ -∗
+  ⌈[∗ map] ps↦li0 ∈ r2av_combine inja' injb', r2a_shared ps li0 @ sat γ⌉ -∗
+
+  (** interesting part starts here *)
+  ⌈r2a_in_inj_inv (r2av_core_a inja' injb') [] @ sat γa⌉ -∗
+  ⌈heap_in_inj_inv (r2av_core_b inja' injb') [] @ sat γb⌉ ==∗⌈sat γ⌉
+  (⌈r2a_in_inj_inv (r2av_combine inja' injb') [] @ sat γ⌉ ∗
+  ([∗ map] ps↦li0 ∈ r2av_core_b inja' injb', r2av_residual γa γb li0)) ∗
+  (** interesting part ends here *)
+
+  memUR_trader (sat γ) (sat γa) r2a_mem r2a_mem ∗
+  heapUR_trader (sat γ) (sat γb) r2a_heap own_heap_s ∗
+  ⌈r2a_memUR_inv ha @ sat γa⌉ ∗
+  ⌈r2a_heapUR_inv hm @ sat γa⌉ ∗
+  ⌈heap_inj_inv_i hm @ sat γb⌉ ∗
+  ⌈heap_inj_inv_s hb @ sat γb⌉ ∗
+  ⌈r2a_shared_auth inja' @ sat γa⌉ ∗
+  ⌈heap_inj_shared_auth injb' @ sat γb⌉.
+Proof.
+  iIntros "#????????? #? ? ?". rewrite /heap_in_inj_inv /r2a_in_inj_inv.
+  have Hempty : ∀ k, k ∈ [] ↔ False by set_solver.
+  setoid_rewrite Hempty. setoid_rewrite bi.False_or.
+  iEval (rewrite r2av_combine_to_b big_sepM_fmap).
+  rewrite (weak_embed_big_sepM _ _ (r2av_core_a _ _)).
+  rewrite !(weak_embed_big_sepM _ _ (r2av_core_b _ _)).
+  iDestruct (big_sepM_r2av_core_a_b_1 with "[] [$] [$]") as "?".
+  { iIntros (???? ->) "(%&%&?&?&?) (%&%&?&?&?)". iDestruct (heapUR_block_excl own_heap_i with "[$] [$]") as %[]. }
+  rewrite -big_sepM_sep.
+  iMod (big_sepM_impl_weak_bupd_frame with "[$] [] [-]") as "[$ ?]".
+  2: iAccu. 2: by iFrame.
+  iIntros "!>" (???). iIntros "(Hta & Htb & ? & Hma & Hmb & ? & Hsha & Hshb)".
+  iIntros "[(% & % & %Heq0 & ? & ? & Hvb) Ha]".
+
+  iDestruct "Ha" as (?[??]%r2av_core_a_lookup_Some) "(%&%&?&?&Hva)" => //=.
+  iMod (heapUR_trade_block with "Htb [$] [$]") as "[? [??]]".
+  iMod (memUR_trade_ptsto_big with "Hta [$] [$]") as "[? [??]]".
+  iDestruct (heapUR_lookup_block (PROP:=uPred rec_to_asmUR) with "Hma [$]") as %?.
+  iDestruct (heapUR_lookup_block (PROP:=uPred heap_injUR) with "Hmb [$]") as %?.
+  simplify_eq.
+  iDestruct (r2av_combine_val_map with "[$] Hsha Hshb [$] Hva Hvb") as "#?". iFrame.
+  iModIntro. erewrite lookup_total_correct => //. rewrite Heq0 Z.add_0_r. iFrame.
+  repeat iSplit => //.
+Qed.
+
+(** Create the two small invariants from the large invariant and the residual. *)
+Lemma r2av_shared_to_ab inja' injb' γa γb γ ha hb hm:
+  r2a_f2i_trader (sat γ) (sat γa) -∗
+  ⌈{sat γa}⌉ -∗ ⌈{sat γb}⌉ -∗
+  memUR_trader (sat γa) (sat γ) r2a_mem r2a_mem -∗
+  heapUR_trader (sat γb) (sat γ) own_heap_s r2a_heap -∗
+  ⌈r2a_memUR_inv ha @ sat γ⌉ -∗
+  ⌈r2a_heapUR_inv hm @ sat γa⌉ -∗
+  ⌈heap_inj_inv_i hm @ sat γb⌉ -∗
+  ⌈r2a_heapUR_inv hb @ sat γ⌉ -∗
+  ⌈[∗ map] ps↦li0 ∈ inja', r2a_shared ps li0 @ sat γa⌉ -∗
+  ⌈[∗ map] ps↦li0 ∈ injb', heap_inj_shared ps li0 @ sat γb⌉ -∗
+  ⌈r2a_shared_auth (r2av_combine inja' injb') @ sat γ⌉ -∗
+
+  (** interesting part starts here *)
+  ⌈r2a_in_inj_inv (r2av_combine inja' injb') [] @ sat γ⌉ -∗
+  ([∗ map] ps↦li0 ∈ r2av_core_b inja' injb', r2av_residual γa γb li0) ==∗
+  ∃ hm',
+  (⌈r2a_in_inj_inv (r2av_core_a inja' injb') [] @ sat γa⌉ ∗
+  ⌈heap_in_inj_inv (r2av_core_b inja' injb') [] @ sat γb⌉) ∗
+  (** interesting part ends here *)
+
+  ⌈{sat γa}⌉ ∗ ⌈{sat γb}⌉ ∗
+  memUR_trader (sat γa) (sat γ) r2a_mem r2a_mem ∗
+  heapUR_trader (sat γb) (sat γ) own_heap_s r2a_heap ∗
+  ⌈r2a_memUR_inv ha @ sat γ⌉ ∗
+  ⌈r2a_heapUR_inv hm' @ sat γa⌉ ∗
+  ⌈heap_inj_inv_i hm' @ sat γb⌉ ∗
+  ⌈r2a_heapUR_inv hb @ sat γ⌉ ∗
+  ⌈r2a_shared_auth (r2av_combine inja' injb') @ sat γ⌉ ∗ ⌜h_static_provs hm' = h_static_provs hm⌝.
+Proof.
+  iIntros "#?????????#Hsa#Hsb???".
+  rewrite /heap_in_inj_inv /r2a_in_inj_inv.
+  have Hempty : ∀ k, k ∈ [] ↔ False by set_solver.
+  setoid_rewrite Hempty. setoid_rewrite bi.False_or.
+  rewrite {2}r2av_combine_to_b big_sepM_fmap.
+  setoid_rewrite (weak_embed_big_sepM _ _ (r2av_core_a _ _)).
+  setoid_rewrite (weak_embed_big_sepM _ _ (r2av_core_b _ _)).
+  setoid_rewrite big_sepM_r2av_core_a_b; try apply _.
+  2: { iIntros (???? ->) "(%&%&?&?&?) (%&%&?&?&?)". iDestruct (heapUR_block_excl own_heap_i with "[$] [$]") as %[]. }
+  iDestruct (big_sepM_sep with "[$]") as "Hm".
+  iApply (big_sepM_impl_bupd_ex_frame with "Hm"). 2: by iFrame.
+  iIntros "!>" (???[?[??]]%r2av_core_b_lookup_Some) "(?&?&Hta&Htb&?&Hinva&Hinvb&?&?&<-) [[%[%Heq0[??]]] [% [% [? [??]]]]]".
+  erewrite lookup_total_correct => //. rewrite Heq0 Z.add_0_r.
+  iDestruct (r2av_split_val_map with "[$] Hsa Hsb [$] [$]") as (bm) "#[? ?]". simpl.
+
+  iApply (weak_embed_bupd_intro (sat γa) with "[$]").
+  iDestruct (heapUR_lookup_block_prov r2a_heap with "Hinva [$]") as %?.
+  iMod (heapUR_update_block r2a_heap with "Hinva [$]") as "[? ?]".
+  iMod (memUR_trade_ptsto_big with "Hta [$] [$]") as "[? [??]]".
+  iIntros "!> Hγa".
+
+  iApply (weak_embed_bupd_intro (sat γb) with "[$]").
+  iMod (heapUR_update_block own_heap_i with "Hinvb [$]") as "[? ?]".
+  iMod (heapUR_trade_block with "Htb [$] [$]") as "[? [??]]".
+  iIntros "!> Hγb".
+
+  iModIntro. iFrame. iSplit!; repeat iSplit => //.
+  - by rewrite h_static_provs_update_block.
+  - apply r2av_core_a_lookup_Some. naive_solver.
+  - done.
+Qed.
+End vertical.
+
+Lemma r2a_bij_vertical m moinit hinit `{!VisNoAng m.(m_trans)} ins f2i :
+  trefines (rec_to_asm ins f2i moinit hinit (rec_heap_inj hinit m))
+           (rec_to_asm ins f2i moinit hinit m).
+Proof.
+  unshelve apply: mod_prepost_combine_bi.
+  set (Σ := #[satΣ heap_injUR; satΣ rec_to_asmUR]).
+  have ? : satG Σ heap_injUR by apply _.
+  have ? : satG Σ rec_to_asmUR by apply _.
+  clearbody Σ.
+  eexists Σ, _, _, _ => γa γb γ.
+  unshelve eexists _.  {
+    exact (λ pl s1 _ s2,
+      ∃ inja injb inj statics, ⌜s1 = s2⌝ ∗ r2a_f2i_trader (sat γ) (sat γa) ∗
+
+        if pl is Env then
+          (* We only require the subseteq here since it makes the
+          initialization easier. *)
+          ⌜r2av_combine inja injb ⊆ inj⌝ ∗ ∃ hm,
+          ⌜h_static_provs hm = statics⌝ ∗
+          ⌈[∗ map] ps↦li0∈inj, r2a_shared ps li0 @ sat γ⌉ ∗
+          ⌈r2a_shared_auth inja @ sat γa⌉ ∗
+          ⌈heap_inj_shared_auth injb @ sat γb⌉ ∗
+          ⌈r2a_in_inj_inv (inja ∖ r2av_core_a inja injb) [] @ sat γa⌉ ∗
+          ⌈heap_in_inj_inv (injb ∖ r2av_core_b inja injb) [] @ sat γb⌉ ∗
+          ([∗ map] ps↦li0 ∈ r2av_core_b inja injb, r2av_residual γa γb li0) ∗
+          ⌈r2a_heapUR_inv hm @ sat γa⌉ ∗
+          ⌈heapUR_inv own_heap_i hm @ sat γb⌉ ∗
+          memUR_trader (sat γa) (sat γ) r2a_mem r2a_mem ∗
+          heapUR_trader (sat γb) (sat γ) own_heap_s r2a_heap ∗
+          (* This proof could be quite a bit simpler without the
+          requirement that the statics stay the same. (It is not used
+          in this proof.) *)
+          ⌈r2a_statics statics @ sat γa⌉ ∗
+          ⌈heap_inj_statics statics @ sat γb⌉ ∗
+          ⌈r2a_statics statics @ sat γ⌉
+        else
+          ⌜inj = r2av_combine inja injb⌝ ∗
+          ⌈[∗ map] ps↦li0∈inja, r2a_shared ps li0 @ sat γa⌉ ∗
+          ⌈[∗ map] ps↦li0∈injb, heap_inj_shared ps li0 @ sat γb⌉ ∗
+          ⌈r2a_shared_auth inj @ sat γ⌉ ∗
+          memUR_trader (sat γ) (sat γa) r2a_mem r2a_mem ∗
+          heapUR_trader (sat γ) (sat γb) r2a_heap own_heap_s ∗
+          ⌈r2a_statics statics @ sat γa⌉ ∗
+          ⌈heap_inj_statics statics @ sat γb⌉ ∗
+          ⌈r2a_statics statics @ sat γ⌉
+          )%I. }
+  split_and!.
+  - move => /= [? []]//= regs mem b ? h ???. apply pp_to_all_forall => ? r Hppex.
+    iIntros "([Hiniti [Hinits Hf2i]] & (?&[Hinv[? #?]]&?) & ?)".
+    iDestruct (r2a_f2i_incl_to_full with "Hf2i") as (f2i_full) "[%Hent #Hf2i_full]".
+    iDestruct (heapUR_lookup_block_big r2a_heap with "Hinv Hinits") as %Hblocks.
+    set staticbs : gmap prov (gmap Z val) :=
+            gset_to_gmap ∅ (h_static_provs h) ∖ hinit.
+    iExists _, _. iSplit!. {
+      apply: satisfiable_bmono; [eapply (r2a_res_init' _ f2i_full)|].
+      iIntros "(Hinvm & Hinvh & ? & ? & ?)".
+      iMod (memUR_alloc_big with "Hinvm") as "[Hinvm $]". { apply map_disjoint_empty_r. }
+      iMod (heapUR_alloc_blocks _ (hinit ∪ staticbs) with "Hinvh") as "[Hinvh Hbs]"; [set_solver|].
+      iDestruct (big_sepM_union with "Hbs") as "[$ ?]";
+        [apply map_disjoint_difference_r'|].
+      rewrite !right_id. iModIntro. iSplit; [iAccu|]. by iApply Hent.
+    } {
+      apply: satisfiable_bmono; [apply heap_inj_init|].
+      iIntros "(? & ? & Hinvi & Hinvs)".
+      iMod (heapUR_alloc_blocks _ (hinit ∪ staticbs) with "Hinvi") as "[Hinvi Hbs]"; [set_solver|].
+      iMod (heapUR_alloc_blocks with "Hinvs") as "[Hinvs $]"; [set_solver|].
+      iDestruct (big_sepM_union with "Hbs") as "[$ ?]";
+        [apply map_disjoint_difference_r'|].
+      rewrite !right_id. iModIntro. iAccu.
+    }
+    iIntros "Hγa Hγb Hγ (?&?&?&Hinvi&?&?) (?&?&?&?&?)".
+    iModIntro. iFrame "#∗". iFrame "#".
+    iExists ∅. rewrite /heap_in_inj_inv /r2a_in_inj_inv !big_sepM_empty. iSplit!.
+    { iApply (r2a_f2i_trader_init with "Hf2i_full [$]"). } {
+      rewrite h_static_provs_heap_from_blocks dom_union_L dom_difference_L.
+      rewrite (comm (R:=(=)) (∪)) difference_union_L.
+      rewrite dom_gset_to_gmap filter_union_L (comm (R:=(=)) (∪)).
+      rewrite subseteq_union_1_L; [set_solver|].
+      rewrite map_subseteq_spec in Hblocks.
+      move => ? /elem_of_filter[?/elem_of_dom[? /Hblocks/h_blocks_lookup_Some[??]]].
+      apply elem_of_filter. split!. by apply elem_of_h_static_provs.
+    }
+    iSplitL "Hinvi Hiniti".
+    + iApply (memUR_trader_init with "[$] [$]").
+    + iApply (heapUR_trader_init_blocks with "[$] [$]").
+  - move => /= ??? [? []//=] ?? b ? h ???. apply pp_to_all_forall => ? r Hppex.
+    iIntros "??? [[[? Hinvm] [Hinvh ?]] ?] (%inja & %injb & %inj & %statics & % & #? & % & %  & % & ? & Hsha & Hshb & Hinja & Hs)". simplify_eq.
+    iDestruct (big_sepL2_length (PROP:=uPred rec_to_asmUR) with "[$]") as %?.
+    iDestruct "Hs" as "(Hinjb & Hbs & ? & ? & Hta & Htb & #Hsa & #Hsb & #Hs)".
+    iDestruct "Hinvh" as "(Hinvh & [%inj' [Hsh Hinj]] & Hs1)".
+    iDestruct (r2a_statics_agree with "Hs Hs1") as %Heq.
+    iDestruct (r2a_shared_lookup_big with "Hsh [$]") as %?.
+
+    iAssert ⌜dom inj' ## dom (injb ∖ r2av_core_b inja injb)⌝%I as %?. {
+      rewrite elem_of_disjoint.
+      iIntros (?[??]%elem_of_dom[??]%elem_of_dom).
+      iDestruct (r2a_in_inj_inv_borrow with "Hinj") as (??) "(?&Hp&?&?)"; [apply not_elem_of_nil|done|].
+      iDestruct (heap_in_inj_inv_borrow with "Hinjb") as (???) "(?&?&?&?)"; [apply not_elem_of_nil|done|].
+      iApply bupd_plainly.
+      iApply (weak_embed_bupd_intro (sat γb) with "[$]").
+      iMod (heapUR_trade_block with "[$] [$] Hp") as "[? [??]]".
+      iDestruct (heapUR_block_excl own_heap_s with "[$] [$]") as %[].
+    }
+
+    (* Technically, h_provs hm should suffice, but it would require more proofs. *)
+    set (X := (dom inja ∪ map_img (fst <$> injb) ∪ h_provs hm)).
+    set (inja' := (r2av_proj_a inj' inja injb X)).
+    set (injb' := (r2av_proj_b inj' inja injb X)).
+
+    have -> : inj' = r2av_combine inja' injb' by
+      apply r2av_combine_proj; [by etrans |done|set_solver..].
+
+    (** Update the small injections  *)
+    iApply (weak_embed_bupd_intro (sat γb) with "[$]").
+    iMod (heap_inj_shared_alloc_big _ injb' with "Hshb") as "[? #Hshbbig]".
+    { apply r2av_proj_b_subseteq. }
+    iIntros "!> Hγb".
+
+    iApply (weak_embed_bupd_intro (sat γa) with "[$]").
+    iMod (r2a_shared_alloc_big _ inja' with "Hsha") as "[? #Hshabig]".
+    { apply r2av_proj_a_subseteq. }
+    iIntros "!> Hγa".
+
+    (** Update the residual *)
+    iMod (r2av_alloc_residual (r2av_core_b inja' injb' ∖ r2av_core_b inja injb) with "[$] [$] [$] [$]") as (hm') "[Hbs' [Hγa [Hγb[?[?%Heqm]]]]]". {
+      move => ? /elem_of_map_img[? /lookup_fmap_Some[? [? ]]]. subst.
+      move => /r2av_core_b_proj_fresh[|/(fresh_map_lookup_Some _ _ _ _)]; set_solver.
+    } {
+      move => ??? /lookup_fmap_Some[[??][? /r2av_core_b_proj_fresh[|??]]]. 1: set_solver.
+      move => /lookup_fmap_Some[[??][? /r2av_core_b_proj_fresh[|??]]]. 1: set_solver. simplify_eq/=.
+      by apply: fresh_map_bij.
+    } { move => ?? /r2av_core_b_proj_fresh[|//]. set_solver. } {
+      apply equiv_empty_L. move => ? /elem_of_filter[? /elem_of_map_img[? /lookup_fmap_Some[l [? ]]]]. subst.
+      move => /r2av_core_b_proj_fresh[//|/fresh_map_is_Block]. 1: set_solver. by destruct l.1.
+    }
+    iDestruct (big_sepM_union_2 with "Hbs Hbs'") as "Hbs".
+    rewrite map_difference_union. 2: { apply r2av_core_b_proj_subseteq. }
+
+    (** Create the small [heap_in_inj_inv]. *)
+    iMod (r2av_shared_to_ab with "[$] Hγa Hγb Hta Htb [$] [$] [$] [$] [$] [$] [$] [$] [$]") as (?) "([??] & ? & ? & ? & ? & ? & ? & ? & ? & ? & %Heqm')".
+
+    iDestruct (r2a_in_inj_inv_combine with "Hinja [$]") as "Hinja".
+    iDestruct (heap_in_inj_inv_combine with "Hinjb [$]") as "Hinjb".
+    erewrite r2av_recombine_a => //. erewrite r2av_recombine_b => //.
+    2: set_solver.
+
+    (** Split the val_in_inj for the arguments. *)
+    iDestruct (r2av_split_val_list with "[$] Hshabig Hshbbig [$] [$]") as (vms) "#[Hv1 ?]".
+    iDestruct (big_sepL2_length (PROP:=uPred rec_to_asmUR) with "Hv1") as %?.
+
+    (** Transfer the traders *)
+    iApply (weak_embed_bupd_intro (sat γb) with "[$]").
+    iMod (heapUR_trader_switch with "[$] [$]") as "[? ?]".
+    iIntros "!> ?".
+    iApply (weak_embed_bupd_intro (sat γa) with "[$]").
+    iMod (r2a_mem_stack_trade with "[$] [$] [$]") as "[? [? ?]]".
+    iMod (memUR_trader_switch with "[$] [$]") as "[? ?]".
+    iIntros "!> ?". iModIntro.
+
+    (** Finish *)
+    iExists b; destruct b; destruct!/=; iFrame.
+    (* We need to be careful here to not accidentally instantiate
+    evars via the [Persistent] typeclass search of [iSplit] for bigops *)
+    all: iSplit; [done|]; iExists vms, _; iFrame "#∗"; iSplit!; rewrite -?Heq ?Heqm' ?Heqm //.
+    + iSplit; [|done]. done.
+    + rewrite right_id. iApply (r2a_f2i_trade_incl with "[$] [$]").
+    + by repeat iSplit.
+    + by iSplit.
+    + by rewrite {1}(list_to_singleton vms).
+    + iSplit; [by iSplit|]. by rewrite {2}(list_to_singleton vms).
+    + done.
+  - move => /= ??? e ???????. apply pp_to_all_forall => ? r Hppex.
+    iIntros "??? [[[? Hinvma] [Hinvha Hva]] Hr] [[Hinvb Hvb] ?] (%inja & %injb & %inj & %statics & % & #? & % & ? & ? & Hsh & Hta & Htb & Hsa & Hsb & #Hs)".
+    iDestruct (big_sepL2_length (PROP:=uPred heap_injUR) with "[$]") as %?.
+    rewrite heap_of_event_event_set_vals_heap vals_of_event_event_set_vals_heap //.
+    iDestruct "Hinvha" as "(Hinvha & [%inja' [Hsha Hinja]] & Hsa1)".
+    iDestruct "Hinvb" as "(Hinvib & Hinvsb & [%injb' [Hshb Hinjb]] & Hsb1 & Hsb2)".
+    iDestruct (r2a_statics_agree with "Hsa Hsa1") as %?.
+    iDestruct (heap_inj_statics_eq with "Hsb1 Hsb2") as %Heq.
+    iDestruct (heap_inj_statics_eq with "Hsb Hsb1") as %?.
+    iDestruct (r2a_shared_lookup_big with "Hsha [$]") as %?.
+    iDestruct (heap_inj_shared_lookup_big with "Hshb [$]") as %?. subst.
+
+    (** Update the large injection *)
+    iApply (weak_embed_bupd_intro (sat γ) with "[$]").
+    iMod (r2a_shared_alloc_big _ (r2av_combine inja' injb') with "Hsh") as "[? #Hshbig]".
+    { subst. by apply r2av_combine_subseteq. }
+    iIntros "!> ?".
+
+    (** Split the small invariants *)
+    iDestruct (r2a_in_inj_inv_split (r2av_core_a inja' injb') with "Hinja") as "[? Hinja]"; [apply r2av_core_a_subseteq|].
+    iDestruct (heap_in_inj_inv_split (r2av_core_b inja' injb') with "Hinjb") as "[? Hinjb]"; [apply r2av_core_b_subseteq|].
+
+    (** Combine the small invariants to get the large invariant. *)
+    iApply (weak_embed_bupd_intro (sat γ) with "[$]").
+    iMod (r2av_shared_from_ab with "[$] [$] [$] [$] [$] [$] [$] [$] [$] [$] [$] [$]") as "[[??][?[?[? [? [? [? [Hsha Hshb]]]]]]]]".
+
+    (** Combine the val_in_inj for the arguments. *)
+    iDestruct (r2av_combine_val_list with "[$] Hsha Hshb [$] [$] [$]") as "#Hvs".
+
+    (** Trade the stack. *)
+    iMod (r2a_mem_stack_trade with "[$] [$] [$]") as "[? [? ?]]".
+
+    (** Transfer the traders *)
+    iMod (memUR_trader_switch with "[$] [$]") as "[? ?]".
+    iMod (heapUR_trader_switch with "[$] [$]") as "[? ?]".
+    iIntros "!> ?". iModIntro.
+
+    (** Finish *)
+    rewrite Heq. destruct e as [? []]; destruct!/=.
+    all: iFrame "#∗".
+    all: iSplit! => //.
+    + by iSplit.
+    + iDestruct "Hr" as "[? _]". iApply (r2a_f2i_trade_incl with "[] [$]"). by iApply r2a_f2i_trader_switch.
+    + by iSplit.
+Qed.
+
+Lemma r2a_bij_vertical_N m moinit hinit `{!VisNoAng m.(m_trans)} ins f2i n:
+  trefines (rec_to_asm ins f2i moinit hinit (rec_heap_inj_N n hinit m))
+           (rec_to_asm ins f2i moinit hinit m).
+Proof. elim: n => //= ??. etrans; [by apply: r2a_bij_vertical|eauto]. Qed.
